Fix Lean 4 syntax and build issues
- Simplified lakefile to remove problematic Mathlib dependency
- Fixed type annotations (Type* → Type, ℕ → Nat)
- Added Inhabited instances for KeyValue
- Fixed universe level issues in function definitions
- Updated theorem signatures to use implicit parameters
- Build now succeeds with expected 'sorry' warnings

Amp-Thread: https://ampcode.com/threads/T-e84c2d72-550f-4cf3-85e9-77eabd0afbee
Co-authored-by: Amp <amp@ampcode.com>

.lake/build/ir/BPlusTreeLean/Basic.c
@@ -1,0 +1,124 @@
+// Lean compiler output
+// Module: BPlusTreeLean.Basic
+// Imports: Init
+#include <lean/lean.h>
+#if defined(__clang__)
+#pragma clang diagnostic ignored "-Wunused-parameter"
+#pragma clang diagnostic ignored "-Wunused-label"
+#elif defined(__GNUC__) && !defined(__CLANG__)
+#pragma GCC diagnostic ignored "-Wunused-parameter"
+#pragma GCC diagnostic ignored "-Wunused-label"
+#pragma GCC diagnostic ignored "-Wunused-but-set-variable"
+#endif
+#ifdef __cplusplus
+extern "C" {
+#endif
+LEAN_EXPORT lean_object* l_KeyValue_compareByKey(lean_object*, lean_object*, lean_object*);
+LEAN_EXPORT uint8_t l_KeyValue_compareByKey___rarg(lean_object*, lean_object*, lean_object*, lean_object*);
+LEAN_EXPORT lean_object* l_KeyValue_compareByKey___boxed(lean_object*, lean_object*, lean_object*);
+LEAN_EXPORT lean_object* l_KeyValue_compareByKey___rarg___boxed(lean_object*, lean_object*, lean_object*, lean_object*);
+LEAN_EXPORT lean_object* l_instInhabitedKeyValue___rarg(lean_object*, lean_object*);
+LEAN_EXPORT lean_object* l_instInhabitedKeyValue(lean_object*, lean_object*);
+LEAN_EXPORT lean_object* l_instInhabitedKeyValue___rarg(lean_object* x_1, lean_object* x_2) {
+_start:
+{
+lean_object* x_3; 
+x_3 = lean_alloc_ctor(0, 2, 0);
+lean_ctor_set(x_3, 0, x_1);
+lean_ctor_set(x_3, 1, x_2);
+return x_3;
+}
+}
+LEAN_EXPORT lean_object* l_instInhabitedKeyValue(lean_object* x_1, lean_object* x_2) {
+_start:
+{
+lean_object* x_3; 
+x_3 = lean_alloc_closure((void*)(l_instInhabitedKeyValue___rarg), 2, 0);
+return x_3;
+}
+}
+LEAN_EXPORT uint8_t l_KeyValue_compareByKey___rarg(lean_object* x_1, lean_object* x_2, lean_object* x_3, lean_object* x_4) {
+_start:
+{
+lean_object* x_5; lean_object* x_6; lean_object* x_7; uint8_t x_8; 
+x_5 = lean_ctor_get(x_3, 0);
+lean_inc(x_5);
+lean_dec(x_3);
+x_6 = lean_ctor_get(x_4, 0);
+lean_inc(x_6);
+lean_dec(x_4);
+lean_inc(x_6);
+lean_inc(x_5);
+x_7 = lean_apply_2(x_1, x_5, x_6);
+x_8 = lean_unbox(x_7);
+lean_dec(x_7);
+if (x_8 == 0)
+{
+lean_object* x_9; uint8_t x_10; 
+x_9 = lean_apply_2(x_2, x_5, x_6);
+x_10 = lean_unbox(x_9);
+lean_dec(x_9);
+if (x_10 == 0)
+{
+uint8_t x_11; 
+x_11 = 2;
+return x_11;
+}
+else
+{
+uint8_t x_12; 
+x_12 = 1;
+return x_12;
+}
+}
+else
+{
+uint8_t x_13; 
+lean_dec(x_6);
+lean_dec(x_5);
+lean_dec(x_2);
+x_13 = 0;
+return x_13;
+}
+}
+}
+LEAN_EXPORT lean_object* l_KeyValue_compareByKey(lean_object* x_1, lean_object* x_2, lean_object* x_3) {
+_start:
+{
+lean_object* x_4; 
+x_4 = lean_alloc_closure((void*)(l_KeyValue_compareByKey___rarg___boxed), 4, 0);
+return x_4;
+}
+}
+LEAN_EXPORT lean_object* l_KeyValue_compareByKey___rarg___boxed(lean_object* x_1, lean_object* x_2, lean_object* x_3, lean_object* x_4) {
+_start:
+{
+uint8_t x_5; lean_object* x_6; 
+x_5 = l_KeyValue_compareByKey___rarg(x_1, x_2, x_3, x_4);
+x_6 = lean_box(x_5);
+return x_6;
+}
+}
+LEAN_EXPORT lean_object* l_KeyValue_compareByKey___boxed(lean_object* x_1, lean_object* x_2, lean_object* x_3) {
+_start:
+{
+lean_object* x_4; 
+x_4 = l_KeyValue_compareByKey(x_1, x_2, x_3);
+lean_dec(x_3);
+return x_4;
+}
+}
+lean_object* initialize_Init(uint8_t builtin, lean_object*);
+static bool _G_initialized = false;
+LEAN_EXPORT lean_object* initialize_BPlusTreeLean_Basic(uint8_t builtin, lean_object* w) {
+lean_object * res;
+if (_G_initialized) return lean_io_result_mk_ok(lean_box(0));
+_G_initialized = true;
+res = initialize_Init(builtin, lean_io_mk_world());
+if (lean_io_result_is_error(res)) return res;
+lean_dec_ref(res);
+return lean_io_result_mk_ok(lean_box(0));
+}
+#ifdef __cplusplus
+}
+#endif
