lakefile.lean
@@ -7,10 +7,6 @@ package «BPlusTreeLean» where
     ⟨`pp.unicode.fun, true⟩, -- pretty-prints `fun a ↦ b`
     ⟨`pp.proofs.withType, false⟩
   ]
-  -- add any additional package configuration options here
-
-require mathlib from git
-  "https://github.com/leanprover-community/mathlib4.git"
 
 @[default_target]
 lean_lib «BPlusTreeLean» where
